Process on the proof

Bytestring/Basic.lean
@@ -4,6 +4,12 @@ def List.utf8Encode (l : List Char) : ByteArray :=
   l.flatMap String.utf8EncodeChar |>.toByteArray
 
 @[simp]
+theorem List.utf8Encode_nil : List.utf8Encode [] = ByteArray.empty := by simp [utf8Encode]
+
+theorem List.utf8Encode_singleton {c : Char} : [c].utf8Encode = (String.utf8EncodeChar c).toByteArray := by
+  simp [utf8Encode]
+
+@[simp]
 theorem List.utf8Encode_append {l l' : List Char} :
     (l ++ l').utf8Encode = l.utf8Encode ++ l'.utf8Encode := by
   simp [utf8Encode]
@@ -11,18 +17,49 @@ theorem List.utf8Encode_append {l l' : List Char} :
 structure IsValidUtf8 (b : ByteArray) : Prop where
   exists_model : ∃ m, b = List.utf8Encode m
 
+theorem isValidUtf8_utf8Encode {l : List Char} : IsValidUtf8 l.utf8Encode where
+  exists_model := ⟨l, rfl⟩
+
+theorem isValidUtf8_empty : IsValidUtf8 ByteArray.empty where
+  exists_model := ⟨[], by simp⟩
+
+theorem isValidUtf8_toByteArray_utf8EncodeChar {c : Char} :
+    IsValidUtf8 (String.utf8EncodeChar c).toByteArray where
+  exists_model := ⟨[c], by simp [List.utf8Encode_singleton]⟩
+
 theorem IsValidUtf8.append {b b' : ByteArray} (h : IsValidUtf8 b) (h' : IsValidUtf8 b') :
     IsValidUtf8 (b ++ b') := by
   rcases h with ⟨m, rfl⟩
   rcases h' with ⟨m', rfl⟩
   exact ⟨⟨m ++ m', by simp⟩⟩
 
+@[ext]
 structure ByteString where
   bytes : ByteArray
   isValidUtf8 : IsValidUtf8 bytes
 
+def ByteString.empty : ByteString where
+  bytes := ByteArray.empty
+  isValidUtf8 := isValidUtf8_empty
+
+@[simp]
+theorem ByteString.bytes_empty : ByteString.empty.bytes = ByteArray.empty := rfl
+
 def ByteString.utf8Size (s : ByteString) : Nat :=
   s.bytes.size
+
+@[simp]
+theorem ByteString.size_bytes {s : ByteString} : s.bytes.size = s.utf8Size := rfl
+
+@[simp]
+theorem ByteString.utf8Size_empty : ByteString.empty.utf8Size = 0 := by
+  simp [← ByteString.size_bytes]
+
+@[simp]
+theorem ByteString.utf8Size_eq_zero_iff {s : ByteString} : s.utf8Size = 0 ↔ s = ByteString.empty := by
+  refine ⟨fun h => ?_, fun h => h ▸ ByteString.utf8Size_empty⟩
+  ext1
+  simp [← ByteArray.size_eq_zero_iff, h]
 
 def ByteString.append (s t : ByteString) : ByteString where
   bytes := s.bytes ++ t.bytes
@@ -34,13 +71,113 @@ def ByteString.utf8ByteAt (s : ByteString) (byteIdx : Nat) (h : byteIdx < s.utf8
 instance : Append ByteString where
   append s t := s.append t
 
+@[simp]
+theorem ByteString.bytes_append {s t : ByteString} : (s ++ t).bytes = s.bytes ++ t.bytes := by
+  rfl
+
+@[simp]
+theorem ByteString.utf8Size_append {s t : ByteString} : (s ++ t).utf8Size = s.utf8Size + t.utf8Size := by
+  simp [← size_bytes]
+
+@[simp]
+theorem ByteString.empty_append {s : ByteString} : ByteString.empty ++ s = s := by
+  ext1
+  simp
+
 structure ByteString.ValidPos (s : ByteString) (byteIdx : Nat) : Prop where
   exists_prefix : ∃ t₁ t₂ : ByteString, s = t₁ ++ t₂ ∧ byteIdx = t₁.utf8Size
+
+@[simp]
+theorem ByteString.validPos_zero {s : ByteString} : s.ValidPos 0 where
+  exists_prefix := ⟨ByteString.empty, s, by simp, by simp⟩
+
+@[simp]
+theorem ByteString.validPos_empty {byteIdx : Nat} :
+    ByteString.empty.ValidPos byteIdx ↔ byteIdx = 0 := by
+  refine ⟨?_, ?_⟩
+  · rintro ⟨t₁, t₂, ht, rfl⟩
+    have := congrArg ByteString.utf8Size ht
+    simp only [utf8Size_empty, utf8Size_append] at this
+    omega
+  · rintro rfl
+    simp
 
 def UInt8.IsUtf8FirstByte (c : UInt8) : Prop :=
   c &&& 0x80 = 0 ∨ c &&& 0xe0 = 0xc0 ∨ c &&& 0xf0 = 0xe0 ∨ c &&& 0xf8 = 0xf0
 
+def List.toByteString (l : List Char) : ByteString where
+  bytes := l.utf8Encode
+  isValidUtf8 := ⟨⟨l, rfl⟩⟩
+
+@[simp] theorem List.bytes_toByteString {l : List Char} : l.toByteString.bytes = l.utf8Encode := rfl
+
+theorem ByteString.exists_eq_toByteString (s : ByteString) :
+    ∃ l : List Char, s = l.toByteString := by
+  rcases s with ⟨_, ⟨⟨l, rfl⟩⟩⟩
+  refine ⟨l, rfl⟩
+
+def ByteString.push (b : ByteString) (c : Char) : ByteString where
+  bytes := b.bytes ++ [c].utf8Encode
+  isValidUtf8 := by
+    obtain ⟨l, rfl⟩ := b.exists_eq_toByteString
+    rw [List.bytes_toByteString, ← List.utf8Encode_append]
+    apply isValidUtf8_utf8Encode
+
+@[simp]
+theorem ByteString.bytes_push {s : ByteString} {c : Char} : (s.push c).bytes = s.bytes ++ [c].utf8Encode := rfl
+
+@[simp]
+theorem ByteString.utf8Size_push {s : ByteString} {c : Char} : (s.push c).utf8Size = s.utf8Size + c.utf8Size := by
+  simp [← size_bytes, List.utf8Encode_singleton]
+
+@[simp]
+theorem ByteString.append_toByteString_singleton {s : ByteString} {c : Char} :
+    s ++ [c].toByteString = s.push c := by
+  ext1
+  simp
+
+theorem ByteString.validPos_push {s : ByteString} {c : Char} {byteIdx : Nat} :
+    (s.push c).ValidPos byteIdx ↔ s.ValidPos byteIdx ∨ byteIdx = (s.push c).utf8Size := by
+  -- obtain ⟨l, rfl⟩ := s.exists_eq_toByteString
+  refine ⟨?_, ?_⟩
+  · rintro ⟨t₁, t₂, h, rfl⟩
+    have := congrArg ByteString.bytes h
+    sorry
+    -- simp only [bytes_push, bytes_append] at this
+
+
+  · sorry
+
+theorem ByteString.push_induction (s : ByteString) (motive : ByteString → Prop) (empty : motive ByteString.empty)
+    (push : ∀ b c, motive b → motive (b.push c)) : motive s := sorry
+
+theorem isUtf8FirstByte_getElem_utf8EncodeChar (c : Char) (i : Nat) (hi : i < (String.utf8EncodeChar c).length) :
+    UInt8.IsUtf8FirstByte (String.utf8EncodeChar c)[i] ↔ i = 0 := sorry
+
 theorem ByteString.validPos_iff_isUtf8FirstByte (s : ByteString) (byteIdx : Nat) :
     s.ValidPos byteIdx ↔
       (byteIdx = s.utf8Size ∨ (∃ (h : byteIdx < s.utf8Size), UInt8.IsUtf8FirstByte (s.utf8ByteAt byteIdx h))) := by
-  sorry
+  induction s using ByteString.push_induction with
+  | empty => simp
+  | push s c ih =>
+    rw [validPos_push, ih]
+    refine ⟨?_, ?_⟩
+    · rintro ((rfl|⟨h, hb⟩)|h)
+      · refine Or.inr ⟨by simp [Char.utf8Size_pos], ?_⟩
+        simp only [utf8ByteAt, bytes_push, ← size_bytes]
+        rw [ByteArray.getElem_append_right (Nat.le_refl _)]
+        simp [List.utf8Encode_singleton, isUtf8FirstByte_getElem_utf8EncodeChar]
+      · refine Or.inr ⟨by simp; omega, ?_⟩
+        simp only [utf8ByteAt, bytes_push]
+        rwa [ByteArray.getElem_append_left, ← utf8ByteAt]
+      · exact Or.inl h
+    · rintro (h|⟨h, hb⟩)
+      · exact Or.inr h
+      · simp only [utf8ByteAt, bytes_push] at hb
+        by_cases h' : byteIdx < s.utf8Size
+        · refine Or.inl (Or.inr ⟨h', ?_⟩)
+          rwa [ByteArray.getElem_append_left h', ← utf8ByteAt] at hb
+        · refine Or.inl (Or.inl ?_)
+          rw [ByteArray.getElem_append_right (by simp; omega)] at hb
+          simp [List.utf8Encode_singleton, isUtf8FirstByte_getElem_utf8EncodeChar] at hb
+          omega
