Bytestring/ByteArray.lean
@@ -20,6 +20,10 @@ theorem ByteArray.data_push {a : ByteArray} {b : UInt8} :
 theorem ByteArray.data_empty : ByteArray.empty.data = #[] := rfl
 
 @[simp]
+theorem ByteArray.size_empty : ByteArray.empty.size = 0 := by
+  simp [← ByteArray.size_data]
+
+@[simp]
 theorem List.data_toByteArray {l : List UInt8} :
     l.toByteArray.data = l.toArray := by
   rw [List.toByteArray]
@@ -29,7 +33,49 @@ theorem List.data_toByteArray {l : List UInt8} :
   fun_induction List.toByteArray.loop a b with simp_all
 
 @[simp]
+theorem List.size_toByteArray {l : List UInt8} :
+    l.toByteArray.size = l.length := by
+  simp [← ByteArray.size_data]
+
+@[simp]
 theorem List.toByteArray_append {l l' : List UInt8} :
     (l ++ l').toByteArray = l.toByteArray ++ l'.toByteArray := by
   ext1
   simp
+
+@[simp]
+theorem List.toByteArray_empty : List.toByteArray [] = ByteArray.empty := rfl
+
+@[simp]
+theorem ByteArray.empty_append {b : ByteArray} : ByteArray.empty ++ b = b := by
+  ext1
+  simp
+
+@[simp]
+theorem ByteArray.size_append {a b : ByteArray} : (a ++ b).size = a.size + b.size := by
+  simp [← size_data]
+
+@[simp]
+theorem ByteArray.size_eq_zero_iff {a : ByteArray} : a.size = 0 ↔ a = ByteArray.empty := by
+  refine ⟨fun h => ?_, fun h => h ▸ ByteArray.size_empty⟩
+  ext1
+  simp [← Array.size_eq_zero_iff, h]
+
+theorem ByteArray.getElem_eq_getElem_data {a : ByteArray} {i : Nat} {h : i < a.size} :
+    a[i] = a.data[i]'(by simpa [← size_data]) := rfl
+
+theorem ByteArray.getElem_append_left {i : Nat} {a b : ByteArray} {h : i < (a ++ b).size}
+    (hlt : i < a.size) : (a ++ b)[i] = a[i] := by
+  simp only [getElem_eq_getElem_data, data_append]
+  rw [Array.getElem_append_left (by simpa)]
+
+theorem ByteArray.getElem_append_right {i : Nat} {a b : ByteArray} {h : i < (a ++ b).size}
+    (hle : a.size ≤ i) : (a ++ b)[i] = b[i - a.size]'(by simp_all; omega) := by
+  simp only [getElem_eq_getElem_data, data_append]
+  rw [Array.getElem_append_right (by simpa)]
+  simp
+
+@[simp]
+theorem List.getElem_toByteArray {l : List UInt8} {i : Nat} {h : i < l.toByteArray.size} :
+    l.toByteArray[i] = l[i]'(by simp_all) := by
+  simp [ByteArray.getElem_eq_getElem_data]
